generated/TLS13.Wire.Generated.ServerHelloBody_extensions.fst
@@ -37,29 +37,29 @@ module LPITE = LowParse.PulseParse.IfThenElse
 
 assume val fits_u64_squash : squash FStar.SizeT.fits_u64
 
-let serverHelloBody_extensions_list_bytesize_nil = LP.serialize_list_nil extension_parser extension_serializer
+let serverHelloBody_extensions_list_bytesize_nil = LP.serialize_list_nil extensionServerHello_parser extensionServerHello_serializer
 
-let serverHelloBody_extensions_list_bytesize_cons x y = LP.serialize_list_cons extension_parser extension_serializer x y; (extension_bytesize_eq (x))
+let serverHelloBody_extensions_list_bytesize_cons x y = LP.serialize_list_cons extensionServerHello_parser extensionServerHello_serializer x y; (extensionServerHello_bytesize_eq (x))
 
 noextract let serverHelloBody_extensions'_parser : LP.parser _ serverHelloBody_extensions' =
-  LP.parse_bounded_vldata_strong 6 65535 (LP.serialize_list _ extension_serializer)
+  LP.parse_bounded_vldata_strong 6 65535 (LP.serialize_list _ extensionServerHello_serializer)
 
 let serverHelloBody_extensions_parser = serverHelloBody_extensions'_parser `LP.parse_synth` synth_serverHelloBody_extensions 
 
 noextract let serverHelloBody_extensions'_serializer : LP.serializer serverHelloBody_extensions'_parser =
-  LP.serialize_bounded_vldata_strong 6 65535 (LP.serialize_list _ extension_serializer)
+  LP.serialize_bounded_vldata_strong 6 65535 (LP.serialize_list _ extensionServerHello_serializer)
 
 let serverHelloBody_extensions_serializer = LP.serialize_synth _ synth_serverHelloBody_extensions serverHelloBody_extensions'_serializer synth_serverHelloBody_extensions_recip ()
 
 let serverHelloBody_extensions_bytesize_eq x = ()
 
 inline_for_extraction let serverHelloBody_extensions'_validator : LPS.validator serverHelloBody_extensions'_parser =
-  PPVD.validate_bounded_vldata_strong 6 65535 (LP.serialize_list _ extension_serializer) (PPLS.validate_list extension_validator ()) (PPBI.leaf_read_bounded_integer_2 fits_u64_squash) fits_u64_squash
+  PPVD.validate_bounded_vldata_strong 6 65535 (LP.serialize_list _ extensionServerHello_serializer) (PPLS.validate_list extensionServerHello_validator ()) (PPBI.leaf_read_bounded_integer_2 fits_u64_squash) fits_u64_squash
 
 let serverHelloBody_extensions_validator = LPC.validate_synth serverHelloBody_extensions'_validator synth_serverHelloBody_extensions
 
 inline_for_extraction let serverHelloBody_extensions'_jumper : LPS.jumper serverHelloBody_extensions'_parser =
-  PPVD.jump_bounded_vldata_strong 6 65535 (LP.serialize_list _ extension_serializer) (PPB.serialized_of_leaf_reader (LP.serialize_bounded_integer (LP.log256' 65535)) (PPBI.leaf_read_bounded_integer_2 fits_u64_squash)) fits_u64_squash
+  PPVD.jump_bounded_vldata_strong 6 65535 (LP.serialize_list _ extensionServerHello_serializer) (PPB.serialized_of_leaf_reader (LP.serialize_bounded_integer (LP.log256' 65535)) (PPBI.leaf_read_bounded_integer_2 fits_u64_squash)) fits_u64_squash
 
 let serverHelloBody_extensions_jumper = LPC.jump_synth serverHelloBody_extensions'_jumper synth_serverHelloBody_extensions
 
@@ -71,24 +71,24 @@ let serverHelloBody_extensions_copyful_synth_inverse () : Lemma (LP.synth_invers
 let read_serverHelloBody_extensions : PPB.copyful_parse serverHelloBody_extensions_vmatch serverHelloBody_extensions_parser serverHelloBody_extensions_conv =
   serverHelloBody_extensions_copyful_synth_injective ();
   serverHelloBody_extensions_copyful_synth_inverse ();
-  assert_norm ((LP.get_parser_kind extension_parser).LP.parser_kind_subkind == Some LP.ParserStrong);
-  assert_norm ((LP.get_parser_kind extension_parser).LP.parser_kind_low > 0);
+  assert_norm ((LP.get_parser_kind extensionServerHello_parser).LP.parser_kind_subkind == Some LP.ParserStrong);
+  assert_norm ((LP.get_parser_kind extensionServerHello_parser).LP.parser_kind_low > 0);
   PPC.copyful_parse_synth
-    (PPVD.copyful_parse_bounded_vldata_strong_payload 6 65535 (LP.serialize_list _ extension_serializer)
-       (PPLS.copyful_parse_list read_extension extension_jumper ())
+    (PPVD.copyful_parse_bounded_vldata_strong_payload 6 65535 (LP.serialize_list _ extensionServerHello_serializer)
+       (PPLS.copyful_parse_list read_extensionServerHello extensionServerHello_jumper ())
        (PPBI.leaf_read_bounded_integer_2 fits_u64_squash) fits_u64_squash)
     synth_serverHelloBody_extensions synth_serverHelloBody_extensions_recip
 
 let free_serverHelloBody_extensions : PPB.free_t serverHelloBody_extensions_vmatch =
-  PPVD.free_vldata_strong 6 65535 (LP.serialize_list _ extension_serializer) (PPVCL.free_vclist (PPB.free_vmatch_conv extension_vmatch extension_conv free_extension))
+  PPVD.free_vldata_strong 6 65535 (LP.serialize_list _ extensionServerHello_serializer) (PPVCL.free_vclist (PPB.free_vmatch_conv extensionServerHello_vmatch extensionServerHello_conv free_extensionServerHello))
 
 let write_serverHelloBody_extensions : PPB.l2r_safe_writer serverHelloBody_extensions_vmatch serverHelloBody_extensions_serializer serverHelloBody_extensions_conv =
   serverHelloBody_extensions_copyful_synth_injective ();
   serverHelloBody_extensions_copyful_synth_inverse ();
-  assert_norm ((LP.get_parser_kind extension_parser).LP.parser_kind_subkind == Some LP.ParserStrong);
-  assert_norm ((LP.get_parser_kind extension_parser).LP.parser_kind_low > 0);
+  assert_norm ((LP.get_parser_kind extensionServerHello_parser).LP.parser_kind_subkind == Some LP.ParserStrong);
+  assert_norm ((LP.get_parser_kind extensionServerHello_parser).LP.parser_kind_low > 0);
   PPC.l2r_safe_writer_synth
-    ((PPVD.l2r_safe_writer_bounded_vldata_strong_payload 6 (LSeqB.mk_seq_sizet 6 fits_u64_squash) 65535 (LSeqB.mk_seq_sizet 65535 fits_u64_squash) 2 2sz (LP.serialize_list _ extension_serializer)
-       (PPLS.l2r_safe_writer_list extension_serializer write_extension ()) fits_u64_squash) <: PPB.l2r_safe_writer _ serverHelloBody_extensions'_serializer _)
+    ((PPVD.l2r_safe_writer_bounded_vldata_strong_payload 6 (LSeqB.mk_seq_sizet 6 fits_u64_squash) 65535 (LSeqB.mk_seq_sizet 65535 fits_u64_squash) 2 2sz (LP.serialize_list _ extensionServerHello_serializer)
+       (PPLS.l2r_safe_writer_list extensionServerHello_serializer write_extensionServerHello ()) fits_u64_squash) <: PPB.l2r_safe_writer _ serverHelloBody_extensions'_serializer _)
     synth_serverHelloBody_extensions synth_serverHelloBody_extensions_recip
 
